

$B \rightarrow B_1 \mid \mid M B_2 \mid B_1 \&\& M B_2 \mid ! B_1 \mid (B_1) \mid E_1 \text{ rel } E_2 \mid \text{true} \mid \text{false}$
 $M \rightarrow \epsilon$

- 1) $B \rightarrow B_1 \mid \mid M B_2$ { $\text{backpatch}(B_1.\text{falselist}, M.\text{instr});$
 $B.\text{truelist} = \text{merge}(B_1.\text{truelist}, B_2.\text{truelist});$
 $B.\text{falselist} = B_2.\text{falselist};$ }
- 2) $B \rightarrow B_1 \&\& M B_2$ { $\text{backpatch}(B_1.\text{truelist}, M.\text{instr});$
 $B.\text{truelist} = B_2.\text{truelist};$
 $B.\text{falselist} = \text{merge}(B_1.\text{falselist}, B_2.\text{falselist});$ }
- 3) $B \rightarrow ! B_1$ { $B.\text{truelist} = B_1.\text{falselist};$
 $B.\text{falselist} = B_1.\text{truelist};$ }
- 4) $B \rightarrow (B_1)$ { $B.\text{truelist} = B_1.\text{truelist};$
 $B.\text{falselist} = B_1.\text{falselist};$ }
- 5) $B \rightarrow E_1 \text{ rel } E_2$ { $B.\text{truelist} = \text{makelist}(\text{nextinstr});$
 $B.\text{falselist} = \text{makelist}(\text{nextinstr} + 1);$
 $\text{gen}(' \text{if } E_1.\text{addr rel.op } E_2.\text{addr goto } _ ');$
 $\text{gen}(' \text{goto } _ ');$ }
- 6) $B \rightarrow \text{true}$ { $B.\text{truelist} = \text{makelist}(\text{nextinstr});$
 $\text{gen}(' \text{goto } _ ');$ }
- 7) $B \rightarrow \text{false}$ { $B.\text{falselist} = \text{makelist}(\text{nextinstr});$
 $\text{gen}(' \text{goto } _ ');$ }
- 8) $M \rightarrow \epsilon$ { $M.\text{instr} = \text{nextinstr};$ }

- 1) $S \rightarrow \text{if } (B) M S_1$ { $\text{backpatch}(B.\text{truelist}, M.\text{instr});$
 $S.\text{nextlist} = \text{merge}(B.\text{falselist}, S_1.\text{nextlist});$ }
- 2) $S \rightarrow \text{if } (B) M_1 S_1 N \text{ else } M_2 S_2$
{ $\text{backpatch}(B.\text{truelist}, M_1.\text{instr});$
 $\text{backpatch}(B.\text{falselist}, M_2.\text{instr});$
 $\text{temp} = \text{merge}(S_1.\text{nextlist}, N.\text{nextlist});$
 $S.\text{nextlist} = \text{merge}(\text{temp}, S_2.\text{nextlist});$ }
- 3) $S \rightarrow \text{while } M_1 (B) M_2 S_1$
{ $\text{backpatch}(S_1.\text{nextlist}, M_1.\text{instr});$
 $\text{backpatch}(B.\text{truelist}, M_2.\text{instr});$
 $S.\text{nextlist} = B.\text{falselist};$
 $\text{gen}(' \text{goto } M_1.\text{instr} ');$ }
- 4) $S \rightarrow \{ L \}$ { $S.\text{nextlist} = L.\text{nextlist};$ }
- 5) $S \rightarrow A$; { $S.\text{nextlist} = \text{null};$ }
- 6) $M \rightarrow \epsilon$ { $M.\text{instr} = \text{nextinstr};$ }
- 7) $N \rightarrow \epsilon$ { $N.\text{nextlist} = \text{makelist}(\text{nextinstr});$
 $\text{gen}(' \text{goto } _ ');$ }
- 8) $L \rightarrow L_1 M S$ { $\text{backpatch}(L_1.\text{nextlist}, M.\text{instr});$
 $L.\text{nextlist} = S.\text{nextlist};$ }
- 9) $L \rightarrow S$ { $L.\text{nextlist} = S.\text{nextlist};$ }